ApcOptimizer.lean
@@ -1,5 +1,6 @@
 -- Root of the `ApcOptimizer` library.
 import ApcOptimizer.Optimizer
+import ApcOptimizer.Sp1Semantics
 import ApcOptimizer.Implementation.JsonParser
 import ApcOptimizer.Utils.Dsl
 import ApcOptimizer.Utils.Size
